ZK_General.ec
@@ -1,50 +1,12 @@
 require import AllCore.
 
-(* Dominique: prob to statement[in language]?
-
-
-*)
 type prob, wit, chal, com, resp, sbits, event.
 
-(*  *)
+
 module type Prover = {
   proc commit(x : prob, w : wit) : com
   proc response(ch : chal) : resp
 }.
-
-(* module type GenProver = { *)
-(*   proc *init() : unit *)
-(*   (* proc rounds() : int *) *)
-(*   proc interact(m : msg) : msg option *)
-(* }. *)
-
-(* module type GenVerifier = { *)
-(*   proc *init() : unit *)
-(*   proc interact(m: msg) : msg option *)
-(*   proc result(): bool *)
-(* } *)
-
-(* module 3ToGen(HV: Verifier3) = { *)
-(*   proc init() = HV.init() *)
-(*   proc interact(m:msg) : msg  *)
-(*   if (i==0) HV.comm *)
-(*   ... *)
-(*   if (i==3) 3ToGen.result = HV.finalmsgreaction(m) *)
-(* } *)
-(* proc result()  = {return 3ToGen.result} *)
-(* } *)
-
-(* module SeqComposeP(P : GenProver) : GenProver = { ... } *)
-
-(* If P is e-sound, then SeqComposeV(HV,n) is e^n-sound 
-
-M(Correct(P, HV : Verifier3)) = Correct(M(P), SeqComposeV(3ToGen(HV) : GenVerifier))
-
-(!P. M(Correct(P, HV)) <= e) = (!P. Correct(M(P), SeqComposeV(HV)) <= e) = (!P. Correct(P, SeqComposeV(HV)))
-
-pros of new approach: more general -> proofs harder
-
-*)
 
 (* AProver, aux in &m of state Pr exper*)
 module type AProver = {
@@ -125,10 +87,7 @@ module Soundness(P : AProver, V : Verifier) = {
 
 
 
-(* ZK -> ZK_Real
-Verifier -> AVerifier
-
- *)
+(* ZK -> ZK_Real, Verifier -> AVerifier *)
 module ZK(P : Prover, V : Verifier) = {
   proc main(Ny : prob, w : wit) = {
     var c,b,r,result;
@@ -221,21 +180,30 @@ end section.
 
 
 
+
+require import AllCore Distr FSet StdRing StdOrder StdBigop List.
+(*---*) import RField RealOrder Bigreal BRA.
+
 require While_Props.
-clone import While_Props as MW with type irt <- (prob),
-                                    type rrt <- event * sbits.
+clone import While_Props as MW with type irt   <- prob,
+                                    type rrt   <- event * sbits,
+                                    type sbits <- sbits.
 import MW.IFB.
 import MW.IFB.IM.
 
-section.
-
 require import Aux.
+
+
+section.
 
 declare module Sim1 : Simulator{DW, W}.
 declare module P : Prover.
 declare module V : Verifier.
 
+op fevent : event.
+
 axiom Sim1_ll : islossless Sim1.run.
+axiom Sim1_run_rew x : hoare[ Sim1.run : (glob Sim1) = x ==> (glob Sim1) = x ].
 
 
 lemma zk_step1 &m E Q p w eps:
@@ -261,25 +229,19 @@ apply oip3;auto.
 qed.
 
 
-op fevent : event.
-
-
-require import AllCore Distr FSet StdRing StdOrder StdBigop List.
-(*---*) import RField RealOrder Bigreal BRA.
-
 lemma zk_step2 &m E Q p ea :
+  E fevent = false =>
   Pr[ W(Sim1).whp((fun x => E (fst x)),p,1,ea,(fevent,witness)) 
            @ &m : E res.`1 /\ Q res.`2 ]  
      = big predT
         (fun i => Pr[Sim1.run(p) @ &m : !E res.`1] ^ i 
          * Pr[ Sim1.run(p) @ &m : E res.`1 /\ Q res.`2] )
         (range 0 ea). 
+move => sev.
 apply (whp_cap_fin_sum Sim1 _ &m (fun x => E (fst x)) (fun x => Q (snd x))).
-admit.
-admit.
-admit.
+apply Sim1_ll. simplify. assumption.
+apply Sim1_run_rew.
 qed.
-
 
 
 lemma big_split_min ['a]:
@@ -301,16 +263,17 @@ lemma zk_step3 &m E Q p w eps ea coeff:
         - Pr[ZK(P,V).main(p,w) @ &m: Q res]| <= eps
   => 0%r < Pr[Sim1.run(p) @ &m : E res.`1]  
   => 0%r <= eps 
-  => exists (eps' : real),  
-     coeff = big predT
+  => coeff = big predT
                (fun i => Pr[Sim1.run(p) @ &m : !E res.`1] ^ i 
                          * Pr[ Sim1.run(p) @ &m : E res.`1])
                (range 0 ea) 
-  => 0%r <= eps' <= eps   /\ 
+  => E fevent = false
+  => exists (eps' : real), 
+    0%r <= eps' <= eps   /\ 
      `|Pr[ W(Sim1).whp(E \o fst,p,1,ea,(fevent,witness)) 
            @ &m : E res.`1 /\ Q res.`2 ]  
          - coeff * Pr[ZK(P,V).main(p,w) @ &m: Q res]| = coeff * eps'.
-proof. move => H0 H1 H2.
+proof. move => H0 H1 H2 coeffeq sev.
 have :  exists (eps' : real),  0%r <= eps' <= eps  
   /\ `|Pr[ Sim1.run(p) @ &m : E res.`1 /\ Q res.`2] 
          / Pr[Sim1.run(p) @ &m : E res.`1] 
@@ -324,12 +287,10 @@ have :  exists (eps' : real),  0%r <= eps' <= eps
         * (Pr[ZK(P,V).main(p,w) @ &m: Q res] + eps')).
 apply (zk_step1 &m). assumption. assumption. assumption.
 elim. move => eps' [H3 [H41 H42 ]].
-exists eps'.  move => coeffeq.
+exists eps'. 
 split. auto.
 apply oip4.
-
 rewrite coeffeq.
-
 have ->: Pr[Sim1.run(p) @ &m : ! E res.`1]
   = 1%r - Pr[Sim1.run(p) @ &m :  E res.`1].
   have ->: 1%r = Pr[Sim1.run(p) @ &m :  true].
@@ -343,14 +304,12 @@ bigi predT
      (1%r - Pr[Sim1.run(p) @ &m : E res.`1]) ^ i *
      Pr[Sim1.run(p) @ &m : E res.`1]) 0 ea.
   apply (big_geq0  Pr[Sim1.run(p) @ &m : E res.`1] _ ea). smt.
-  smt.
-
- 
+  smt. 
 case (Pr[ Sim1.run(p) @ &m : E res.`1 /\ Q res.`2] 
       = Pr[Sim1.run(p) @ &m : E res.`1]  
         * (Pr[ZK(P,V).main(p,w) @ &m: Q res] + eps')).
 progress. rewrite /(\o).
-rewrite zk_step2.
+rewrite zk_step2. assumption.
 rewrite H. simplify.
 have : bigi predT
   (fun (i : int) =>
@@ -370,7 +329,7 @@ have : Pr[ Sim1.run(p) @ &m : E res.`1 /\ Q res.`2]
           * (Pr[ZK(P,V).main(p,w) @ &m: Q res] - eps').
 smt.
 progress. rewrite /(\o).
-rewrite zk_step2.
+rewrite zk_step2. assumption.
 rewrite H. simplify.
 have : bigi predT
   (fun (i : int) =>
@@ -384,6 +343,73 @@ rewrite mulr_suml.
 rewrite - big_split_min.
 simplify. smt.
 timeout 20. smt.
+qed.
+
+
+module Iter(Sim1 : Simulator)  = {
+  module WI = W(Sim1)
+  proc run(Ny : prob, ea : int, E : event * sbits -> bool) = {
+    var r;
+    r <@ WI.whp(E,Ny,1,ea,(fevent,witness));
+    return r;
+  }
+}.
+
+
+lemma zk_final &m E Q p w eps ea coeff:
+   `|Pr[ Sim1.run(p) @ &m : E res.`1 /\ Q res.`2]
+      / Pr[Sim1.run(p) @ &m : E res.`1] 
+        - Pr[ZK(P,V).main(p,w) @ &m: Q res]| <= eps
+  => 0%r < Pr[Sim1.run(p) @ &m : E res.`1]  
+  => 0%r <= eps 
+  => coeff = big predT
+               (fun i => Pr[Sim1.run(p) @ &m : !E res.`1] ^ i 
+                         * Pr[ Sim1.run(p) @ &m : E res.`1])
+               (range 0 ea) 
+  => E fevent = false
+  =>
+     `|Pr[ Iter(Sim1).run(p,ea,E \o fst) 
+           @ &m : E res.`1 /\ Q res.`2 ]  
+         - coeff * Pr[ZK(P,V).main(p,w) @ &m: Q res]| <= eps.
+move => H1 H2 H3 H4 H5.
+have ->: 
+  Pr[Iter(Sim1).run(p, ea, E \o fun (p0 : event * sbits) => p0.`1) @ &m :
+     E res.`1 /\ Q res.`2]
+  = Pr[ W(Sim1).whp(E \o fst,p,1,ea,(fevent,witness)) 
+           @ &m : E res.`1 /\ Q res.`2 ] .  
+ byequiv (_: _==> ={res}). proc*.
+inline Iter(Sim1).run. sp. wp. 
+call (_: ={glob Sim1}). simplify. sim. 
+skip. smt. auto. auto.
+have : coeff <= 1%r. 
+rewrite H4.
+have ->: Pr[Sim1.run(p) @ &m : ! E res.`1]
+  = 1%r - Pr[Sim1.run(p) @ &m :  E res.`1].
+  have ->: 1%r = Pr[Sim1.run(p) @ &m :  true].
+  byphoare. apply Sim1_ll. auto. auto.
+  have ->: Pr[Sim1.run(p) @ &m : true] = Pr[Sim1.run(p) @ &m : E res.`1]
+   + Pr[Sim1.run(p) @ &m : !E res.`1]. rewrite Pr[mu_split E res.`1]. 
+  simplify. smt. smt.
+  have : 
+bigi predT
+  (fun (i : int) =>
+     (1%r - Pr[Sim1.run(p) @ &m : E res.`1]) ^ i *
+     Pr[Sim1.run(p) @ &m : E res.`1]) 0 ea <= 1%r.
+  apply (big_leq1  Pr[Sim1.run(p) @ &m : E res.`1] _ ea). smt.
+  smt.
+move => H6.
+have : exists eps', 0%r <= eps' <= eps /\ `|Pr[W(Sim1).whp(E \o fun (p0 : event * sbits) => p0.`1, p, 1, ea,
+                 (fevent, witness)) @ &m :
+     E res.`1 /\ Q res.`2] -
+  coeff * Pr[ZK(P, V).main(p, w) @ &m : Q res]| 
+  = coeff * eps'.
+apply (zk_step3 &m E Q p w eps ea coeff H1 H2 H3).
+auto. assumption.
+elim.
+move => eps' [eps'p1 epsp2].
+apply (ler_trans (coeff * eps')).
+smt.
+smt.
 qed.
 
 
